pcuic/theories/PCUICTyping.v
@@ -35,7 +35,7 @@ Fixpoint isArity T :=
   | _ => False
   end.
 
-Definition type_of_constructor mdecl (cdecl : ident * term * nat) (c : inductive * nat) (u : list Level.t) :=
+Definition type_of_constructor mdecl (cdecl : constructor_body) (c : inductive * nat) (u : list Level.t) :=
   let mind := inductive_mind (fst c) in
   subst0 (inds mind u mdecl.(ind_bodies)) (subst_instance_constr u (snd (fst cdecl))).
 
